WIP

noc/NOC_setup.v
@@ -4,47 +4,191 @@ Require Import Router.
 Require Import Types.
 From Coq Require Import Arith Lia Program.
 From Equations Require Import Equations.
+Require Import Coq.Vectors.Fin.
 
 Module Type NOC_data.
   Parameter nocsize: nat.
+  Axiom nocprop: nocsize>1.
 End NOC_data.
 
-Module NOCSetup(ND:NOC_data).
+Module NOCSetup(ND:NOC_data)(MyTypes: Typesize).
 Import ND. 
-Import Types.
-Definition regno := (Nat.sub nocsize 1).
+Module NOC_type := Types(MyTypes).
+Import NOC_type.
+Definition interfacesize := Nat.mul nocsize 2. 
+Definition regno := Nat.add nocsize (Nat.sub nocsize 1).
 
-Inductive reg_t := reg_ (n: Vect.index regno).
-Inductive rule_name_t :=
-  | route0_r
-  | route1_r
-  | route2_r
-  | route3_r.
 
-(* Inductive rule_name_t := router_ (n: Vect.index nocsize). *)
+Inductive reg_t : nat -> Type :=
+  | reg_ : forall num, Fin.t num -> reg_t num.
 
-  (* Axiom index_of_nat_never_none : forall n, index_of_nat regno n <> None. 
-Equations reg (n : nat) : reg_t :=  
-  reg n :=
-  match index_of_nat regno n with
-  | Some m => reg_ m
-  | None => absurd (index_of_nat regno n = None) index_of_nat_never_none 
+  Inductive rule_name_t : nat -> Type :=
+  | rule_ : forall num, Fin.t num -> rule_name_t num.
+
+  Inductive ext_fn_t : nat -> Type :=
+  | ex_ : forall num, Fin.t num -> ext_fn_t num.
+
+  Print Fin.
+
+(* Inductive reg_t: nat->Type := reg_ (n: Vect.index regno).
+Inductive rule_name_t := rule_ (n: Vect.index nocsize).
+
+Inductive ext_fn_t := ex_ (n: Vect.index interfacesize). *)
+
+Module MyRegs <: Registers.
+Definition reg_t:=reg_t regno.
+Definition ext_fn_t:= ext_fn_t interfacesize.
+End MyRegs.
+
+Module Routerfns:= Router(MyRegs)(MyTypes).        
+Import Routerfns.
+
+Locate "<".
+Print lt.
+Locate "<=".
+Print le.
+Locate "<>".
+Print not. 
+
+ (* Fixpoint nat_to_fin {n : nat} (m : nat) : option (Fin.t n) :=
+  match n return option (Fin.t n) with
+  | 0 => None (* No valid index if the bound is 0 *)
+  | S n' => match m with
+            | 0 => Some Fin.F1 (* The 0th index corresponds to Fin.F1 *)
+            | S m' => match nat_to_fin m' with
+                      | Some fin' => Some (Fin.FS fin') (* Successor index *)
+                      | None => None
+                      end
+            end
   end. *)
-(* 
- Definition router n :=
+
+  Check Nat.nlt_0_r.
+  Check Fin.of_nat_lt.
+  Definition nat_to_fin {n : nat} (i : nat) (pf : i < n) : Fin.t n :=
+  Fin.of_nat_lt pf.
+  Check Nat.nlt_0_r.
+
+  Example example_fin_auto : 0 < 7.
+Proof.
+  lia. (* auto and info_auto dont work for some numbers*)
+Qed.
+
+Checl
+Compute Fin.of_nat_lt example_fin_auto.
+  Compute @nat_to_fin nocsize 6.
+Check Nat.lt_0_succ.
+
+Fail Check rule_ nocsize Fin.F1.
+Equations to_action' (nocsize:nat) (H: 1<=nocsize) (rl : rule_name_t nocsize) : uaction (reg_t regno) (ext_fn_t interfacesize) := 
+(* to_action 0 H _ := { }; *)
+(* to_action 1 (le_S n H1) _ with H1 := {} ;  *)
+to_action' 1 H (rule_ nocsize Fin.F1) := routestartfn 0 (reg_ regno Fin.F1) (reg_ regno (Fin.FS Fin.F1)) 
+(ex_ interfacesize Fin.F1) (ex_ interfacesize (Fin.FS Fin.F1)) ;
+to_action' _ H r with r := 
+to_action' nocsize H (rule_ nocsize Fin.F1) => routecenterfn 0 (reg_ ) (reg_ 1) (ex_ 0) (ex_ 1).
+
+(* to_action nocsize H (rule_ nocsize n) := routecenterfn n (reg_ n) (reg_ (Nat.add nocsize n) ex_ 2n ex_ 2n+1) *)
+
+Equations to_action (nocsize:nat) (H: 2<=nocsize) (rl : rule_name_t nocsize) : uaction (reg_t regno) (ext_fn_t interfacesize) := 
+(* to_action 0 H _ := { }; *)
+to_action 1 (le_S n H1) _ with H1 := {} ; 
+to_action 2 H r with r := 
+| rule_ 1 => routeendfn 1 (reg_ 1) (reg_fn (Nat.add nocsize 1)) (ex_ 2) (ex_ 3)
+to_action _ H r with r := 
+to_action' (Nat.sub nocsize 1) H rl.
+
+
+  let idx_nat := index_to_nat idx in
+  if Nat.eqb idx_nat 0 then
+    routestartfn 0 (reg_  indices 1)
+  else if Nat.eqb idx_nat regno then
+    let idx' := index_of_nat (Nat.sub idx_nat - 1) in
+    routeendfn regno (reg_ idx')
+  else
+    let idx' := index_of_nat (Nat.sub idx_nat - 1) in
+    routecenterfn idx_nat (reg_ idx') (reg_ idx).
+
+ 
+(* Fixpoint nat_to_fin {n : nat} (m : nat) : option (Fin.t n) :=
+  match n return option (Fin.t n) with
+  | 0 => None (* No valid index if the bound is 0 *)
+  | S n' => match m with
+            | 0 => Some Fin.F1 (* The 0th index corresponds to Fin.F1 *)
+            | S m' => match nat_to_fin m' with
+                      | Some fin' => Some (Fin.FS fin') (* Successor index *)
+                      | None => None
+                      end
+            end
+  end.
+
+Compute @nat_to_fin 4 2.
+
+Inductive reg_t (num : nat) : Type :=
+  | reg_ : Fin.t num -> reg_t num.
+
+Inductive rule_name_t (num : nat) : Type :=
+  | rule_ : Fin.t num -> rule_name_t num.
+
+Inductive ext_fn_t (num : nat) : Type :=
+  | ext_ : Fin.t num -> ext_fn_t num.
+
+
+(*How is num correctly determined*)
+Definition reg_fn (num : nat) (n : nat) : option (reg_t num) :=  
+    match Fin.of_nat n num with
+    | inleft fin_idx => Some (reg_ num fin_idx)  (* Valid index, return register *)
+    | inright _ => None  (* Index out of bounds, return None *)
+    end.
+
+Definition rule_fn (num : nat) (n : nat) : option (rule_name_t num) :=
+    match Fin.of_nat n num with
+    | inleft fin_idx => Some (rule_ num fin_idx)  (* Valid index, return register *)
+    | inright _ => None  (* Index out of bounds, return None *)
+    end.
+
+Definition e_fn (num : nat) (n : nat) : option (ext_fn_t num) :=
+    match Fin.of_nat n num with
+    | inleft fin_idx => Some (ext_ num fin_idx)  (* Valid index, return register *)
+    | inright _ => None  (* Index out of bounds, return None *)
+    end.
+
+Search Fin.t. 
+Compute rule_ 2 (Fin.FS Fin.F1).
+Check rule_fn nocsize 0.
+(* Axiom rego_ge_1 : regno >= 1. (*
+  unfold regno.
+  induction nocsize eqn:H.
+  - set (H1 := nocprop).
+    rewrite H in H1.
+    unfold ">"%nat in H1.
+    apply Nat.nlt_succ_diag_l in H1.
+    contradiction.
+  - apply IHn. *)
+Definition reg_of_nat (n:nat) :reg_t.
+  set (a := index_of_nat regno n).
+  destruct a eqn:H.
+  - exact (reg_ i).
+  - unfold a in H.
+    destruct regno eqn:H1.
+    + admit.
+    + simpl in H.
+    unfold index_of_nat in H.
+    Admitted.
+
+Print index_of_nat.
+Definition reg_of_nat n :=
+  reg_ (match index_of_nat regno n with
+        | Some n => n
+        | None => thisone
+        end). *)
+
+ (* Definition router n :=
   router_ (match index_of_nat nocsize n with
         | Some n => n
         | None => thisone
-        end).  
-  *)
-Module MyRegs <: Registers.
-  Definition reg_t:=reg_t.
-End MyRegs.
-
-
-Module Routerfns:= Router(MyRegs).        
-Import Routerfns.
-Compute index 3.
+        end).   *)
+ 
+(* Compute index 3.
 Compute index_of_nat nocsize 1.
 
 
@@ -59,16 +203,9 @@ Fixpoint list_seq_index (N : nat) : list (index N) :=
   match N with
   | O => nil
   | S N' => cons (thisone) (list_seq_index_anotherone (list_seq_index N'))
-  end.
-
-  Fixpoint get_nth_item_default {A : Type} (l : list A) (n : nat) (default : A) : A :=
-    match l, n with
-    | [], _ => default
-    | x :: _, 0 => x
-    | _ :: xs, S n' => get_nth_item_default xs n' default
-    end.
+  end. 
   
-(* Fixpoint get_nth_item_fin {A : Type} (l : list A) (n : Fin.t regno) : A :=
+Fixpoint get_nth_item_fin {A : Type} (l : list A) (n : Fin.t regno) : A :=
   match l with
   | [] => match n with end (* This case is impossible due to the dependent type *)
   | x :: xs =>
@@ -78,31 +215,39 @@ Fixpoint list_seq_index (N : nat) : list (index N) :=
     end
   end. *)
 
+Module MyRegs <: Registers.
+Definition reg_t:=reg_t regno.
+Definition ext_fn_t:= ext_fn_t regno.
+End MyRegs.
 
-Definition indices := list_seq_index regno.
-Compute indices.
-Check get_nth_item_default indices 1.
-(* Definition get_reg (n: nat): reg_t := reg_ (get_nth_item_default indices n). *)
+Module Routerfns:= Router(MyRegs)(MyTypes).        
+Import Routerfns.
 
-(* Fixpoint give_index (n: nat) : index nocsize :=
-  match n with
-  | 0 => thisone
-  | S n' => anotherone (give_index n')
-  end. *)
+Check rule_fn.
 
-(* Equations to_action (rl : rule_name_t) : uaction reg_t empty_ext_fn_t := 
-to_action (router_ idx) :=
+Definition to_action (rl: rule_name_t nocsize) := 
+match rl with
+| (rule_fn nocsize 0) => routestartfn 0 reg_fn regno 0 reg_fn regno 1 extfn interfacesize 0 extfn interfacesize 1
+| rule_ => routecenterfn 1 r1 r2 r5 extfn_3 extfn_4
+| rule_ => routecenterfn 2 r2 r3 r6 extfn_5 extfn_6
+| rule_ => routeendfn 3 r3 r7 extfn_7 extfn_8
+end.
+
+
+Equations to_action
+ (rl : rule_name_t nocsize) : uaction (reg_t regno) (ext_fn_t interfacesize) := 
+to_action (rule_ nocsize) :=
   let idx_nat := index_to_nat idx in
   if Nat.eqb idx_nat 0 then
-    routestartfn 0 (reg_ get_nth_item_default indices 1)
+    routestartfn 0 (reg_  indices 1)
   else if Nat.eqb idx_nat regno then
     let idx' := index_of_nat (Nat.sub idx_nat - 1) in
     routeendfn regno (reg_ idx')
   else
     let idx' := index_of_nat (Nat.sub idx_nat - 1) in
-    routecenterfn idx_nat (reg_ idx') (reg_ idx). *)
+    routecenterfn idx_nat (reg_ idx') (reg_ idx).
 
-
+ *)
 
 
 
